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Problem - V (Chocolate Problem)
(A small insight to Representation Theory) Prove that every finite group G is isomorphic to a
subgroup of GLn(R) for some n.

Hint: Think about an action of Sn on Rn, where n = |G|.

Proof. Consider the map φ : Sn → K, defined by:

φ(P ) = EP (i),i for P ∈ Sn,

where Ei,j denotes the n× n matrix with 1 in the (i, j)-th position and 0 elsewhere.

To show that φ is a homomorphism, we need to verify that:

φ(P ◦ P ′) = φ(P ) · φ(P ′) for all P, P ′ ∈ Sn.

Let P, P ′ ∈ Sn. Then:

φ(P ◦ P ′) = EP◦P ′(i),i = EP (P ′(i)),P ′(i).

On the other hand, using the definition of φ:

φ(P ) · φ(P ′) = EP (i),i · EP ′(i),i.

Thus, we have shown that φ(P ◦ P ′) = φ(P ) · φ(P ′), confirming that φ is a homomorphism. Next,
we show that φ is bijective:

1. Injectivity: Suppose φ(P ) = φ(P ′), i.e., EP (i),i = EP ′(i),i for all i. This implies that
the positions of the 1’s in the matrices EP (i),i and EP ′(i),i are the same. Therefore, the
permutations P and P ′ must agree, so P = P ′. Hence, φ is injective.

2. Surjectivity: For every permutation matrix M ∈ K, we need to find a permutation P ∈ Sn
such that φ(P ) = M . By the definition of φ, φ(P ) = EP (i),i. Since M is a permutation
matrix, it corresponds to some permutation P ∈ Sn. Therefore, for every M ∈ K, there
exists a permutation P ∈ Sn such that φ(P ) =M . Hence, φ is surjective.

Since φ is both a homomorphism and bijective, we conclude that:
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φ : Sn → K is an isomorphism.

Therefore, we have:

Sn ∼= K ≤ GLn(R).

Claim: The composition of two injective homomorphisms is an injective homomorphism.

Proof: Let G, H, and K be groups, and let φ : G → H and ψ : H → K be homomorphisms.
Assume that both φ and ψ are injective.

We want to show that the composition ψ ◦ φ : G → K is also injective. That is, if (ψ ◦ φ)(g1) =
(ψ ◦ φ)(g2) for some g1, g2 ∈ G, then we must show that g1 = g2.

(ψ ◦ φ)(g1) = (ψ ◦ φ)(g2) =⇒ ψ(φ(g1)) = ψ(φ(g2))

Since ψ is injective, we get that:

φ(g1) = φ(g2)

Next, since φ is injective, we get that:

g1 = g2

Thus, ψ ◦ φ is injective.

Now, we need to show that ψ ◦ φ is a homomorphism.

For all g1, g2 ∈ G, we need to verify that:

(ψ ◦ φ)(g1g2) = (ψ ◦ φ)(g1)(ψ ◦ φ)(g2).

Since φ and ψ are homomorphisms, we know that:

φ(g1g2) = φ(g1)φ(g2) and ψ(φ(g1)φ(g2)) = ψ(φ(g1))ψ(φ(g2)).

Thus,

(ψ ◦ φ)(g1g2) = ψ(φ(g1g2)) = ψ(φ(g1)φ(g2)) = ψ(φ(g1))ψ(φ(g2)) = (ψ ◦ φ)(g1)(ψ ◦ φ)(g2).

Therefore, ψ ◦ φ is a homomorphism. Therefore, the composition of injective homomorphisms is
an injective homomorphism.

Now using this and Cayley’s theorem, we get the theorem.
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